src/syntax.v
@@ -18,8 +18,13 @@ Declare Scope Usuba_var.
 Delimit Scope Usuba_var with ua_var.
 
 Coercion ExpVar : var >-> expr.
+Coercion Var_e : ident >-> arith_expr.
 Coercion Const_e : nat >-> arith_expr.
+
+Definition c x := Const x None.
+Coercion c : nat >-> expr.
 Coercion Var : ident >-> var.
+Coercion Id_s : string >-> ident.
 
 Notation "x '&' y" := (Log And (x)%ua_expr (y)%ua_expr) (at level 87, left associativity) : Usuba_expr.
 Notation "x 'xor' y" := (Log Xor (x)%ua_expr (y)%ua_expr) (at level 87, left associativity) : Usuba_expr.
@@ -27,43 +32,88 @@ Notation "x '<<' y" := (Shift Lshift (x)%ua_expr (y)%ua_aexpr) (at level 87, lef
 Notation "x '>>' y" := (Shift Rshift (x)%ua_expr (y)%ua_aexpr) (at level 87, left associativity) : Usuba_expr.
 Notation "x '<<<' y" := (Shift Lrotate (x)%ua_expr (y)%ua_aexpr) (at level 87, left associativity) : Usuba_expr.
 Notation "x '>>>' y" := (Shift Rrotate (x)%ua_expr (y)%ua_aexpr) (at level 87, left associativity) : Usuba_expr.
+Notation "x '+' y"   := (Arith Add (x)%ua_expr (y)%ua_expr) (at level 50, left associativity) : Usuba_expr.
+Notation "x '-' y"   := (Arith Sub (x)%ua_expr (y)%ua_expr) (at level 50, left associativity) : Usuba_expr.
+Notation "x '*' y"   := (Arith Mul (x)%ua_expr (y)%ua_expr) (at level 40, left associativity) : Usuba_expr.
+Notation "x '/' y"   := (Arith Div (x)%ua_expr (y)%ua_expr) (at level 40, left associativity) : Usuba_expr.
+Notation "f '@' '[' x , .. , y ']'" := (Fun (f)%string (ECons ((x)%ua_expr : expr) .. (ECons ((y)%ua_expr : expr) Enil) ..)) (at level 75, no associativity) : Usuba_expr.
+Notation "'[' x , .. , y ']'" := (Tuple (ECons ((x)%ua_expr : expr) .. (ECons ((y)%ua_expr : expr) Enil) ..)) (at level 87, no associativity) : Usuba_expr.
 
-Notation "v '[' e ']'" := (Index (v)%ua_var (e)%ua_aexpr) (at level 88, left associativity) : Usuba_var.
+Notation "x '+' y"   := (Op_e Add (x)%ua_aexpr (y)%ua_aexpr) (at level 50, left associativity) : Usuba_arith_expr.
+Notation "x '-' y"   := (Op_e Sub (x)%ua_aexpr (y)%ua_aexpr) (at level 50, left associativity) : Usuba_arith_expr.
+Notation "x '*' y"   := (Op_e Mul (x)%ua_aexpr (y)%ua_aexpr) (at level 40, left associativity) : Usuba_arith_expr.
+Notation "x '/' y"   := (Op_e Div (x)%ua_aexpr (y)%ua_aexpr) (at level 40, left associativity) : Usuba_arith_expr.
 
-Notation "a '<=' b ';' tl" := (Dcons (Eqn (a)%ua_var (b)%ua_expr false) tl)
+Notation "v '[' e ']'" := (Index (v)%ua_var  (e)%ua_aexpr) (at level 61, left associativity) : Usuba_var.
+Notation "v '[' e ']'" := (Index (v)%ua_var  (e)%ua_aexpr) (at level 61, left associativity) : Usuba_expr.
+Notation "t '[' e ']'" := (Array (t)%ua_type (e)%ua_aexpr) (at level 61, left associativity) : Usuba_type.
+
+Notation " a '<|-' b" := (Eqn (a)%ua_var (b)%ua_expr false)
+    (at level 89, right associativity) : Usuba_eqn.
+
+Notation " a '<:-' b" := (Eqn (a)%ua_var (b)%ua_expr true)
+    (at level 89, right associativity) : Usuba_eqn.
+
+(* Notation "'(' a1 , .. , a2 ')' '<-' b" := (Eqn (cons (a1)%ua_var .. (cons (a2)%ua_var nil) ..) (b)%ua_expr false)
     (at level 90, right associativity) : Usuba_eqn.
 
-Notation "a '<:=' b ';' tl" := (Dcons (Eqn (a)%ua_var (b)%ua_expr true) tl)
-    (at level 90, right associativity) : Usuba_eqn.
-    
-Notation "a '<:=' b ';'" := (a <:= b ; Dnil)%ua_eqn
-    (at level 89, no associativity) : Usuba_eqn.
-(* Notation "a '<=' b ';'" := (a <= b ; Dnil)%ua_eqn
-    (at level 89, no associativity) : Usuba_eqn. *)
+Notation "'(' a1 , .. , a2 ')' '<:-' b" := (Eqn (cons (a1)%ua_var .. (cons (a2)%ua_var nil) ..) (b)%ua_expr true)
+    (at level 90, right associativity) : Usuba_eqn. *)
 
-Notation "hd ',' tl" :=
-    ((hd)%ua_var_decl ++ (tl)%ua_var_decl)
-        (at level 90, right associativity) : Usuba_var_decl.
+Notation "'for' var 'in' s 'to' e 'do' e1 ; .. ; e2 'done'" :=
+    (Loop var (s)%ua_aexpr (e)%ua_aexpr (Dcons (e1)%ua_eqn .. (Dcons (e2)%ua_eqn Dnil) ..) nil)
+    (at level 90, right associativity) : Usuba_eqn.
 
 Notation " var ':' typ" :=
-    ({| VD_ID := (var)%string; VD_TYP := (typ)%ua_type ; VD_OPTS := nil |}::nil)
-        (at level 89, no associativity) : Usuba_var_decl.
+    ({| VD_ID := (var)%string; VD_TYP := (typ)%ua_type ; VD_OPTS := nil |})
+        (at level 70, no associativity) : Usuba_var_decl.
 
-Notation "'node' name 'args' var_decl 'returns' var_decl2 'vars' var_decl3 'let' eqns 'tel'" :=
+Notation "'node' name 'args' var_decl1 , .. , var_decl1b 'returns' var_decl2 , .. , var_decl2b 'vars' var_decl3 'let' x ; .. ; y 'tel'" :=
     {|
         ID := name;
-        P_IN := (var_decl)%ua_var_decl;
-        P_OUT := (var_decl2)%ua_var_decl;
+        P_IN := (cons (var_decl1)%ua_var_decl .. (cons (var_decl1b)%ua_var_decl nil) ..)%ua_var_decl;
+        P_OUT := (cons (var_decl2)%ua_var_decl .. (cons (var_decl2b)%ua_var_decl nil) ..)%ua_var_decl;
         OPT := No_opt;
-        NODE := Single (var_decl3)%ua_var_decl (eqns)%ua_eqn
+        NODE := Single (var_decl3)%ua_var_decl (Dcons (x)%ua_eqn .. (Dcons (y)%ua_eqn Dnil) ..)
     |} (at level 90).
+
+Notation "'table' name 'args' var_decl1 , .. , var_decl1b 'returns' var_decl2 , .. , var_decl2b 'let' x ; .. ; y 'tel' " :=
+    {|
+        ID := name;
+        P_IN := (cons (var_decl1)%ua_var_decl .. (cons (var_decl1b)%ua_var_decl nil) ..)%ua_var_decl;
+        P_OUT := (cons (var_decl2)%ua_var_decl .. (cons (var_decl2b)%ua_var_decl nil) ..)%ua_var_decl;
+        OPT := No_opt;
+        NODE := Table (cons x .. (cons y nil) ..)
+    |} (at level 90).
+
+Definition v8 : typ := Uint (Varslice (Id_s "D")) (Mvar (Id_s "m")) 8.
+Definition b16  : typ := Uint Bslice (Mint 1) 16.
+Definition b8   : typ := Uint Bslice (Mint 1) 8.
+Definition b1   : typ := Uint Bslice (Mint 1) 1.
+Definition b32  : typ := Uint Bslice (Mint 1) 32.
+Definition b64  : typ := Uint Bslice (Mint 1) 64.
+Definition b128 : typ := Uint Bslice (Mint 1) 128.
+Definition b256 : typ := Uint Bslice (Mint 1) 256.
+Definition b512 : typ := Uint Bslice (Mint 1) 512.
+
+Definition input : string := "input".
+Definition output : string := "output".
+Definition out : string := "out".
+Definition i : string := "i".
+Definition o : string := "o".
+Definition key : string := "key".
+Definition plain : string := "plain".
+Definition cipher : string := "cipher".
+Definition tmp : string := "tmp".
 
 Definition test : string := "test".
 Definition a : string := "a".
 Definition b : string := "b".
 
-Definition node1 := node test args (a : Nat) returns (b : Nat) vars nil 
-    let (Var b [ Const_e 1 ])%ua_var :: nil <:= ExpVar (Var a); tel.
+Definition node1 := node test args a : Nat returns b : Nat vars nil 
+    let 
+        ( b [ 1 ])%ua_var :: nil <:- ExpVar (Var a)
+    tel.
 
 Definition f : ident := "f"%string.
 Definition x : ident := "x"%string.
@@ -73,8 +123,5 @@ Definition refresh : ident := "refresh"%string.
 
 Definition f_node := node f args (x : Uint Vslice (Mint 32) 1) returns (y: Uint Vslice (Mint 32) 1) vars nil
     let
-        Var y :: nil <:= ((x <<< 5) & Fun refresh (ECons x Enil)) xor (x <<< 1);
+        Var y :: nil <:- ((x <<< 5) & Fun refresh (ECons x Enil)) xor (x <<< 1)
     tel.
-
-Print f_node.
-
