src/examples/arch.v
@@ -1,0 +1,129 @@
+Require Import Bool.
+Require Import PeanoNat.
+From Usuba Require Import usuba_sem.
+
+Definition ARCH_ADD_default  (d : dir) : option (nat -> nat -> nat) :=
+    match d with
+        _ => None
+    end.
+Definition ARCH_SUB_default  (d : dir) : option (nat -> nat -> nat) :=
+    match d with
+        _ => None
+    end.
+Definition ARCH_DIV_default  (d : dir) : option (nat -> nat -> nat) :=
+    match d with
+        _ => None
+    end.
+Definition ARCH_MOD_default  (d : dir) : option (nat -> nat -> nat) :=
+    match d with
+        _ => None
+    end.
+Definition ARCH_MUL_default  (d : dir) : option (nat -> nat -> nat) :=
+    match d with
+        _ => None
+    end.
+
+Fixpoint land (len n1 n2 : nat) :=
+    match len with
+    | 0 => 0
+    | S len' =>
+        let tl := land len' (n1 / 2) (n2 / 2) in
+        if Nat.eqb (n1 mod 2) 1 && Nat.eqb (n2 mod 2) 1
+        then 1 + tl * 2
+        else tl * 2
+    end.
+
+Fixpoint lor (len n1 n2 : nat) :=
+    match len with
+    | 0 => 0
+    | S len' =>
+        let tl := lor len' (n1 / 2) (n2 / 2) in
+        if Nat.eqb (n1 mod 2) 1 || Nat.eqb (n2 mod 2) 1
+        then 1 + tl * 2
+        else tl * 2
+    end.
+
+Fixpoint lxor (len n1 n2 : nat) :=
+    match len with
+    | 0 => 0
+    | S len' =>
+        let tl := lxor len' (n1 / 2) (n2 / 2) in
+        if Bool.eqb (Nat.eqb (n1 mod 2) 1) (Nat.eqb (n2 mod 2) 1)
+        then tl * 2
+        else 1 + tl * 2
+    end.
+    
+Definition ARCH_NOT_default  (d : dir) : option (nat -> nat) :=
+    match d with
+        _ => None
+    end.
+
+Definition ARCH_AND_default  (d : dir) : option (nat -> nat -> nat) :=
+    match d with
+        | DirH l => Some (land l)
+        | DirV l => Some (land l)
+        | DirB => Some (land 1)
+        | _ => None
+    end.
+
+Definition ARCH_OR_default   (d : dir) : option (nat -> nat -> nat) :=
+    match d with
+        | DirH l => Some (lor l)
+        | DirV l => Some (lor l)
+        | DirB => Some (lor 1)
+        | _ => None
+    end.
+
+Definition ARCH_XOR_default  (d : dir) : option (nat -> nat -> nat) :=
+    match d with
+        | DirH l => Some (lxor l)
+        | DirV l => Some (lxor l)
+        | DirB => Some (lxor 1)
+        | _ => None
+    end.
+
+Definition ARCH_ANDN_default (d : dir) : option (nat -> nat -> nat) :=
+    match d with
+        _ => None
+    end.
+
+Definition ARCH_LSHIFT_default  (n : nat) (d : dir) : option (nat -> nat) :=
+    match d with
+        _ => None
+    end.
+Definition ARCH_RSHIFT_default  (n : nat) (d : dir) : option (nat -> nat) :=
+    match d with
+        _ => None
+    end.
+Definition ARCH_RASHIFT_default (n : nat) (d : dir) : option (nat -> nat) :=
+    match d with
+        _ => None
+    end.
+Definition ARCH_LROTATE_default (n : nat) (d : dir) : option (nat -> nat) :=
+    match d with
+        _ => None
+    end.
+Definition ARCH_RROTATE_default (n : nat) (d : dir) : option (nat -> nat) :=
+    match d with
+        _ => None
+    end.
+
+Definition default_arch : architecture := {|
+    ARCH_ADD := ARCH_ADD_default;
+    ARCH_SUB := ARCH_SUB_default;
+    ARCH_DIV := ARCH_DIV_default;
+    ARCH_MOD := ARCH_MOD_default;
+    ARCH_MUL := ARCH_MUL_default;
+
+    ARCH_NOT  := ARCH_NOT_default;
+    ARCH_AND  := ARCH_AND_default;
+    ARCH_OR   := ARCH_OR_default;
+    ARCH_XOR  := ARCH_XOR_default;
+    ARCH_ANDN := ARCH_ANDN_default;
+
+    ARCH_LSHIFT  := ARCH_LSHIFT_default;
+    ARCH_RSHIFT  := ARCH_RSHIFT_default;
+    ARCH_RASHIFT := ARCH_RASHIFT_default;
+    ARCH_LROTATE := ARCH_LROTATE_default;
+    ARCH_RROTATE := ARCH_RROTATE_default;
+|}.
