src/extract.v
@@ -1,6 +1,6 @@
 Require Import List.
 Require Import ZArith.
-From Usuba Require Import usuba_AST.
+From Usuba Require Import usuba_AST collect clean.
 Require Extraction.
 Require Import ExtrOcamlNativeString.
 
@@ -8,5 +8,5 @@ Extraction Language OCaml.
 
 
 Extract Inductive bool => bool [ true false ].
-Extract Inductive list => "list" [ "[]" "(::)" ].
-Extraction "usuba" prog.
+Extract Inductive list => "list" [ "[]" "(::)" ]. 
+Extraction "usuba" clean_prog.
