src/usuba_ASTProp.v
@@ -1,0 +1,15 @@
+From Usuba Require Import usuba_AST.
+
+Lemma ident_beq_refl:
+    forall x, ident_beq x x = true.
+Proof.
+    intro x; rewrite ident_beq_eq; reflexivity.
+Qed.
+
+Lemma ident_eq_dec:
+    forall x y : ident, { x = y } + { x <> y}.
+Proof.
+    intros x y; case_eq (ident_beq x y); intro H; [> left | right].
+    2: rewrite <- Bool.not_true_iff_false in H.
+    all: rewrite ident_beq_eq in H; assumption.
+Qed.
