src/usuba_semProp.v
@@ -20,7 +20,7 @@ Lemma simpl_form_preserve_prod:
 Proof.
     move=> form; induction form as [|[|[|hd'']] tl HRec]; simpl; trivial.
     + rewrite <- HRec; clear HRec.
-        unfold muln, muln_rec; rewrite PeanoNat.Nat.mul_1_l; reflexivity.
+        unfold muln, muln_rec; rewrite Nat.mul_1_l; reflexivity.
     + rewrite <- HRec; reflexivity.
 Qed.
 
@@ -30,11 +30,11 @@ Lemma prod_list_append:
 Proof.
     move=> l1; induction l1 as [|hd l1 HRec]; simpl; move=> l2.
     {
-        unfold muln, muln_rec; rewrite PeanoNat.Nat.mul_1_l; reflexivity.
+        unfold muln, muln_rec; rewrite Nat.mul_1_l; reflexivity.
     }
     {
         rewrite HRec.
-        unfold muln, muln_rec; rewrite PeanoNat.Nat.mul_assoc; reflexivity.
+        unfold muln, muln_rec; rewrite Nat.mul_assoc; reflexivity.
     }
 Qed.
 
@@ -48,16 +48,16 @@ Proof.
     induction ctxt1 as [|[n1 v1] ctxt1 HRec1]; simpl.
     {
         move=> ctxt2; induction ctxt2 as [|[n v] tl HRec]; simpl; trivial.
-        case (String.eqb x n).
+        case (ident_beq x n).
         + discriminate.
         + assumption.
     }
     {
         move=> ctxt2.
-        case (String.eqb x n1); auto.
+        case (ident_beq x n1); auto.
         induction ctxt2 as [|[n2 v2] ctxt2 HRec2]; simpl.
         + discriminate.
-        + case (String.eqb x n2).
+        + case (ident_beq x n2).
             - move=> HEq; inversion HEq; reflexivity.
             - assumption.
     }
@@ -73,14 +73,14 @@ Proof.
 Qed.
 
 Theorem linearize_map_CoIL {A : Type} :
-    forall l1 l2, @linearize_list_value A (map CoIL l1) l2 = (map CoIL l1) ++ l2.
+    forall l1 l2, @linearize_list_value A (List.map CoIL l1) l2 = (List.map CoIL l1) ++ l2.
 Proof.
     move=> l1 l2; induction l1 as [|hd l1 HRec]; simpl; trivial.
     rewrite HRec; reflexivity.
 Qed.
 
 Theorem eval_var_linearize_fixpoint:
-    forall ctxt v acc l, eval_var ctxt v acc = Some l -> linearize_list_value l nil = l.
+    forall ctxt v acc l, eval_var v ctxt acc = Some l -> linearize_list_value l nil = l.
 Proof.
     move=> ctxt; induction v as [v|v HRec ae|v HRec ae1 ae2|v HRec aeL]; simpl; move=> acc l.
     {
@@ -125,6 +125,21 @@ Proof.
 Qed.
 
 (* take n property *)
+
+Lemma take_n_sum {A : Type} :
+    forall l l2: list A, forall n, length l = n -> take_n n (l ++ l2) = Some (l, l2).
+Proof.
+    move=> l l2; induction l as [|hd tl HRec]; simpl.
+    {
+        move=> n <-; simpl; reflexivity.
+    }
+    {
+        move=> [|n] HEq; simpl.
+        by discriminate.
+        rewrite HRec; trivial.
+        inversion HEq; reflexivity.
+    }
+Qed.
 
 Lemma take_n_all {A : Type} :
     forall l : list A, forall n, length l = n -> take_n n l = Some (l, nil).
@@ -173,6 +188,147 @@ Proof.
     }
 Qed.
 
+Lemma take_n_soundness2 { A : Type} :
+    forall i l,
+        i <= length l ->
+        exists l1 l2, @take_n (option A) i (List.map Some l) = Some (List.map Some l1, map Some l2) /\ l = l1 ++ l2 /\ length l1 = i.
+Proof.
+    move=> i; induction i as [|i HRec]; simpl.
+    {
+        move=> l _.
+        exists nil; exists l; auto.
+    }
+    {
+        move=> [|hd tl]; simpl.
+        {
+            discriminate.
+        }
+        specialize HRec with tl.
+        move=> Hlt; move: HRec.
+        impl_tac.
+        {
+            apply ltnSE; assumption.
+        }
+        move=> [l1 [l2 [TakeEq [EqAppend LengthEq]]]].
+        rewrite TakeEq.
+        exists (hd::l1); exists l2.
+        simpl.
+        rewrite LengthEq.
+        repeat split; trivial.
+        rewrite EqAppend.
+        simpl; reflexivity.
+    }
+Qed.
+
+Lemma try_take_n_all { A : Type} :
+    forall i l,
+        i = length l ->
+        @try_take_n A i l = (l, IoLR A nil).
+Proof.
+    move=> i; induction i as [|i HRec]; simpl.
+    {
+        move=> []; simpl; trivial.
+        by discriminate.
+    }
+    {
+        move=> [|hd tl]; simpl.
+        by discriminate.
+        specialize HRec with tl.
+        move=> HEq; move: HRec.
+        impl_tac.
+        + inversion HEq; reflexivity.
+        + move=> ->; reflexivity.
+    }
+Qed.
+
+Lemma try_take_n_soundness { A : Type} :
+    forall i l1 l2,
+        i = length l1 ->
+        @try_take_n A i (l1 ++ l2) = (l1, IoLR A l2).
+Proof.
+    move=> i l1 l2; move: l1; induction i as [|i HRec]; simpl.
+    {
+        move=> []; simpl; trivial.
+        by discriminate.
+    }
+    {
+        move=> [|hd tl]; simpl.
+        by discriminate.
+        specialize HRec with tl.
+        move=> HEq; move: HRec.
+        impl_tac.
+        + inversion HEq; reflexivity.
+        + move=> ->; reflexivity.
+    }
+Qed.
+
+(* build_ctxt and auxiliairies properties *)
+
+
+Theorem build_ctxt_aux_take_n_soundness:
+    forall d iL_tl n iL,
+        length iL = n ->
+        iL_tl <> nil ->
+        build_ctxt_aux_take_n n (CoIR d (iL ++ iL_tl) None::nil) d
+            = Some (iL, CoIR d iL_tl None::nil).
+Proof.
+    intros d iL_tl n; induction n as [|n HRec]; simpl.
+    all: intro iL; destruct iL as [|hd iL]; simpl; trivial.
+    1-2: discriminate.
+    rewrite internal_dir_dec_lb0; trivial.
+    intro H; inversion H as [HEq]; clear H.
+    rewrite try_take_n_soundness; trivial.
+    destruct iL_tl; trivial.
+    intro H; exfalso; apply H; reflexivity.
+Qed.
+
+Theorem build_ctxt_aux_take_n_soundness2:
+    forall d n iL,
+        length iL = n ->
+        n <> 0 ->
+        build_ctxt_aux_take_n n (CoIR d iL None::nil) d
+            = Some (iL, nil).
+Proof.
+    intros d n iL LengthEq; simpl.
+    unfold build_ctxt_aux_take_n.
+    rewrite internal_dir_dec_lb0; trivial.
+    rewrite try_take_n_all; auto.
+    destruct n; trivial.
+    intro H; exfalso; apply H; auto.
+Qed.
+
+(* properties about undefined *)
+
+Lemma length_undefined {A : Type} :
+    forall n, length (@undefined A n) = n.
+Proof.
+    intro n; induction n as [|n HRec]; simpl; auto.
+Qed.
+
+Lemma undefined_sum {A : Type}:
+    forall n1 n2,
+        @undefined A (n1 + n2) = undefined n1 ++ undefined n2.
+Proof.
+    intros n n2; induction n as [|n HRec]; simpl; trivial.
+    rewrite HRec; reflexivity.
+Qed.
+
+Lemma undefined_lemma {A : Type}:
+    forall n1 n2,
+    concat (map (fun _=> @undefined A n2) (@undefined A n1)) = undefined (n2 * n1)%coq_nat.
+Proof.
+    intros n1 n2; induction n1 as [|n1 HRec]; simpl.
+    {
+        rewrite Nat.mul_0_r; auto.
+    }
+    {
+        rewrite Nat.mul_succ_r.
+        rewrite Nat.add_comm.
+        rewrite undefined_sum.
+        rewrite HRec; reflexivity.
+    }
+Qed.
+
 (* split_into_segments properties *)
 
 Lemma split_into_segments_soundness {A : Type} :
@@ -218,9 +374,53 @@ Proof.
     }
 Qed.
 
+Lemma split_into_segments_soundness2 {A : Type} :
+    forall i1 i2 l,
+        length l = i1 * i2 ->
+        exists l', @split_into_segments (option A) i1 i2 (List.map Some l) = Some (List.map (List.map Some) l') /\
+            Forall (fun l => length l = i2) l' /\
+            List.concat l' = l /\ length l' = i1.
+Proof.
+    move=> i1 i2; induction i1 as [|i1 HRec]; simpl.
+    {
+        move=> l.
+        unfold muln, muln_rec.
+        rewrite Nat.mul_0_l.
+        destruct l; simpl.
+        2: by discriminate.
+        move=> _; exists nil; simpl.
+        auto.
+    }
+    {
+        move=> l length_eq.
+        pose (p:= take_n_soundness2 i2 l); move: p.
+        impl_tac.
+        {
+            rewrite length_eq; clear.
+            rewrite mulSnr.
+            apply leq_addl.
+        }
+        move=> [l1 [l2 [HEq1 [HEq2 LengthEq]]]].
+        rewrite HEq1.
+        symmetry in HEq2; destruct HEq2.
+        specialize HRec with l2; move: HRec; impl_tac.
+        {
+            rewrite mulSnr in length_eq.
+            refine (length_app_eq _ _ _ _ LengthEq _).
+            rewrite addnC.
+            assumption.
+        }
+        move=> [l [-> [HForall [concat_eq length_eq3]]]].
+        exists (l1::l); simpl.
+        rewrite concat_eq.
+        repeat split; auto.
+    }
+Qed.
+
+
 Lemma split_into_segments_1_r {A : Type}:
     forall l : list A, forall n,
-        length l = n -> split_into_segments n 1 l = Some (map (fun i => [:: i]) l).
+        length l = n -> split_into_segments n 1 l = Some (List.map (fun i => [:: i]) l).
 Proof.
     move=> l; induction l as [|hd l HRec]; simpl.
     by move=> n <-; simpl; reflexivity.
@@ -237,4 +437,59 @@ Proof.
     simpl.
     move=> l n length_eq.
     rewrite take_n_all; trivial.
+Qed.
+
+
+Theorem split_into_segments_undefined {A : Type} :
+    forall n1 n2,
+        split_into_segments n1 n2 (@undefined A (n1 * n2)) = Some (map (fun _=> undefined n2) (@undefined A n1)).
+Proof.
+    intro n1; induction n1 as [|n1 HRec]; simpl; trivial.
+    intro; rewrite undefined_sum.
+    rewrite take_n_sum.
+    2: exact (length_undefined _).
+    rewrite HRec; reflexivity.
+Qed.
+    
+(* other lemmas *)
+
+Theorem get_access_AAll:
+    forall n l, length l = n -> n <> 0 -> get_access (map Some l) AAll (n::nil) = Some l.
+Proof.
+    intros n l lengthEq NotZero; simpl.
+    rewrite map_length; rewrite lengthEq.
+    rewrite PeanoNat.Nat.mod_same; trivial; simpl.
+    rewrite PeanoNat.Nat.div_same; trivial; simpl.
+    rewrite split_into_segments_1_r.
+    {
+        clear; induction l as [|hd tl HRec]; simpl; trivial.
+        rewrite HRec; reflexivity.
+    }
+    rewrite map_length; assumption.
+Qed.
+
+Theorem remove_option_from_list_map_Some {A : Type}:
+    forall l, @remove_option_from_list A (map Some l) = Some l.
+Proof.
+    intro l; induction l as [|hd tl HRec]; simpl; trivial.
+    rewrite HRec; reflexivity.
+Qed.
+
+Theorem list_map2_soundness {A B C : Type}:
+    forall (f : A -> B -> C) l1 l2, length l1 = length l2 ->
+        exists l3, length l3 = length l1 /\ list_map2 f l1 l2 = Some l3.
+Proof.
+    intros f l1; induction l1 as [|h1 t1 HRec]; simpl.
+    {
+        intro l2; destruct l2; simpl.
+        + intro; exists nil; auto.
+        + discriminate.
+    }
+    {
+        intro l2; destruct l2 as [|h2 t2]; simpl.
+        { discriminate. }
+        intro H; inversion H as [length_eq].
+        destruct (HRec _ length_eq) as [l3 [<- ->]].
+        exists (f h1 h2::l3); auto.
+    }
 Qed.
